First complete draft of REPL implementation

compiler/bootstrap/translation/compiler64ProgScript.sml
@@ -292,7 +292,7 @@ Proof
 QED
 
 val compiler_for_eval_alt =
-  “compiler_for_eval (x,y,z)”
+  “compiler_for_eval (id,c,decs)”
   |> SIMP_CONV std_ss [backendTheory.compile_inc_progs_for_eval_eq,
                        compiler_for_eval_def, EVAL “x64_config.reg_count”,
                        backendTheory.ensure_fp_conf_ok_def,
@@ -313,41 +313,123 @@ val r = translate compiler_for_eval_alt;
 
 (* fun eval_prim env s1 decs s2 bs ws = Eval [env,s1,decs,s2,bs,ws] *)
 val _ = append_prog
-  “[Dlet (Locs (POSN 1 2) (POSN 2 30))
-      (Pvar "eval_prim")
-      (Fun "env" (Fun "s1" (Fun "decs" (Fun "s2" (Fun "bs" (Fun "ws"
-         (App Eval [Var (Short "env"); Var (Short "s1");
-                    Var (Short "decs"); Var (Short "s2");
-                    Var (Short "bs"); Var (Short "ws")])))))))]”
+  “[Dlet (Locs (POSN 1 2) (POSN 2 21)) (Pvar "eval_prim")
+     (Fun "x" (Mat (Var (Short "x"))
+       [(Pcon NONE [Pvar "env"; Pvar "s1"; Pvar "decs";
+                    Pvar "s2"; Pvar "bs"; Pvar "ws"],
+         App Eval [Var (Short "env"); Var (Short "s1"); Var (Short "decs");
+                   Var (Short "s2"); Var (Short "bs"); Var (Short "ws")])]))]”
 
-(* TODO: define eval function *)
-(* TODO: define check_and_tweak function *)
-(* TODO: define report_error function *)
-(* TODO: define report_exn function *)
+Datatype:
+  eval_res = Compile_error 'a | Eval_result 'b 'c | Eval_exn 'd 'e
+End
+
+val _ = register_type “:('a,'b,'c,'d,'e) eval_res”;
+
+val _ = (append_prog o process_topdecs) `
+  fun eval (s1,next_gen) (env,id) decs =
+    case compiler_for_eval (id,s1,decs) of
+      None => Compiler_error "ERROR: failed to compile input"
+    | Some (s2,bs,ws) =>
+        let
+          val new_env = eval_prim (env,s1,decs,s2,bs,ws)
+        in Eval_result (new_env,(next_gen+1,0)) (s2,next_gen+1) end
+        handle e => Eval_exn e (s2,next_gen+1) `
+
+val exn_msg_dec = process_topdecs ‘
+  val _ = TextIO.print "ERROR: top-level exception"’
+
+Definition report_exn_def:
+  report_exn e = ^exn_msg_dec
+End
+
+val _ = (next_ml_names := ["report_exn"]);
+val r = translate report_exn_def;
+
+Definition report_error_def:
+  report_error msg =
+    [Dlet (Locs UNKNOWNpt UNKNOWNpt) Pany
+       (App Opapp
+          [Var (Long "TextIO" (Short "print"));
+           Lit (StrLit (explode msg))])]
+End
+
+val _ = (next_ml_names := ["report_error"]);
+val r = translate report_error_def;
+
+val read_next_dec =
+  “[Dlet (Locs UNKNOWNpt UNKNOWNpt) Pany
+       (App Opapp
+          [App Opderef [Var (Long "REPL" (Short "readNextString"))];
+           Con NONE []])]”
+
+Definition check_and_tweak_def:
+  check_and_tweak decs types input_str =
+    let all_decs = decs ++ ^read_next_dec in
+      case infertype_prog types all_decs of
+      | Success new_types => Success (all_decs, new_types)
+      | Failure (loc,msg) =>
+          Failure (concat [msg; implode " at "; locs_to_string input_str loc])
+End
+
+val _ = (next_ml_names := ["check_and_tweak"]);
+val r = translate check_and_tweak_def;
 
 val _ = (append_prog o process_topdecs) `
   fun repl parse types conf env decs input_str =
     (* input_str is passed in here only for error reporting purposes *)
     case check_and_tweak decs types input_str of
-      Error msg => repl parse types conf env (report_error msg) ""
+      Failure msg => repl parse types conf env (report_error msg) ""
     | Success (safe_decs, new_types) =>
       (* here safe_decs are guaranteed to not crash;
          the last declaration of safe_decs calls !REPL.readNextString *)
       case eval conf env safe_decs of
-        CompileError msg => repl parse types conf env (report_error msg) ""
-      | EvalException e  => repl parse types conf env (report_exn e) ""
-      | EvalResult new_env =>
+        Compile_error msg => repl parse types conf env (report_error msg) ""
+      | Eval_exn e new_conf => repl parse types new_conf env (report_exn e) ""
+      | Eval_result new_env new_conf =>
         (* check whether the program that ran has loaded in new input *)
         if !REPL.isEOF then () (* exit if there is no new input *) else
           let val new_input = !REPL.nextString in
             (* if there is new input: parse the input and recurse *)
             case parse new_input of
-              Error msg        => repl parse types conf env (report_error msg) ""
-            | Success new_decs => repl parse new_types conf new_env new_decs new_input
+              Inl msg      => repl parse types new_conf env (report_error msg) ""
+            | Inr new_decs => repl parse new_types new_conf new_env new_decs new_input
           end `
 
+Definition candle_prog_def:
+  candle_prog = DROP (LENGTH basis) repl_prog
+End
+
+Theorem repl_prog_eq_basis_candle:
+  repl_prog = basis ++ candle_prog
+Proof
+  EVAL_TAC
+QED
+
+val r = translate (candle_prog_def |> CONV_RULE (RAND_CONV EVAL));
+
+Definition init_types_def:
+  init_types (u:unit) =
+    case infertype_prog init_config (basis ++ candle_prog) of
+    | Failure _ => init_config
+    | Success t => t
+End
+
+val _ = (next_ml_names := ["init_types"]);
+val r = translate init_types_def;
+
 val _ = (append_prog o process_topdecs) `
-  fun run_interactive_repl cl = () (* TODO: call repl *) `
+  fun run_interactive_repl cl =
+    let
+      val parse = compiler64Prog.compiler_parse_cml_input
+      val types = init_types ()
+      val conf = (decodeProg.read_inc_config "config_enc_str.txt", 1)
+      val env = repl_init_env
+      val decs = []
+      val input_str = ""
+    in
+      repl parse types conf env decs input_str
+    end`
 
 Definition has_repl_flag_def:
   has_repl_flag cl ⇔ MEM (strlit "--repl") cl ∨ MEM (strlit "--candle") cl
